Functionnal correctness example

specs/experimental/Spec.Seq.Lib.fst
@@ -17,7 +17,7 @@ type lbytes n = s:bytes{length s = U32.v n}
 val create: #a:Type -> sz:U32.t -> v:a -> s:seq a{length s = U32.v sz}
 let create #a s v = Seq.create #a (U32.v s) v
 
-val upd: #a:Type -> s:seq a -> i:U32.t{U32.v i < length s} -> 
+val upd: #a:Type -> s:seq a -> i:U32.t{U32.v i < length s} ->
 	 v:a -> s':seq a{length s' = length s}
 let upd #a s i v = Seq.upd #a s (U32.v i) v
 
@@ -36,9 +36,9 @@ let seq_length (#a:Type) (s:seq a) = U32.uint_to_t (length s)
 val blit: #a:Type ->
 	s1:seq a -> ind_s1:U32.t{U32.v ind_s1 <= length s1} ->
 	s2:seq a -> ind_s2:U32.t{U32.v ind_s2 <= length s2} ->
-	len:U32.t{U32.v ind_s1 + U32.v len <= length s1 /\ 
+	len:U32.t{U32.v ind_s1 + U32.v len <= length s1 /\
 		  U32.v ind_s2 + U32.v len <= length s2} ->
-	Tot (res:seq a{length res = length s2}) 
+	Tot (res:seq a{length res = length s2})
 
 #reset-options "--z3rlimit 30"
 
@@ -48,10 +48,53 @@ let blit #a s1 ind_s1 s2 ind_s2 len =
     let f2 = slice s1 ind_s1 (ind_s1 +^ len)  in
     t1 @| f2 @| t3
 
-val update_slice: #a:Type -> s:seq a -> i:U32.t -> l:U32.t{U32.v i + U32.v l <= length s} -> 
+
+
+assume val f: #a:Type -> l:UInt32.t -> (s:lseq a l) -> lseq a l
+
+val update_slice: #a:Type -> s:seq a -> i:U32.t -> l:U32.t{U32.v i + U32.v l <= length s} ->
 		  f: (s:lseq a l -> s:lseq a l) -> Tot (r:seq a{length r = length s})
-let update_slice #a s i l f = 
+
+let update_slice #a s i l f =
     let s1 = slice s 0ul i in
     let s2 = slice s i (i +^ l) in
     let s3 = slice s (i +^ l) (seq_length s) in
     s1 @| (f s2) @| s3
+
+open FStar.HyperStack.ST
+open FStar.Buffer
+
+module ST = FStar.HyperStack.ST
+
+#reset-options "--z3rlimit 15"
+
+assume val f_st : (buf: Buffer.buffer UInt8.t) -> l:UInt32.t{Buffer.length buf = UInt32.v l} ->
+  Stack unit
+  (requires (fun h -> Buffer.live h buf))
+  (ensures  (fun h0 _ h1 -> live h1 buf /\ modifies_1 buf h0 h1 /\ (as_seq h1 buf == (f #UInt8.t l (as_seq h0 buf)))))
+
+val update_slice_st_f : s:buffer UInt8.t -> ls:UInt32.t{Buffer.length s = UInt32.v ls} -> i:U32.t -> l:U32.t{U32.v i + U32.v l <= UInt32.v ls} -> Stack unit
+  (requires (fun h -> live h s))
+  (ensures (fun h0 _ h1 -> live h0 s /\ live h1 s /\ modifies_1 s h0 h1
+                      /\ (let s1 = slice (as_seq h0 s) 0ul i in
+                        let s1' = slice (as_seq h1 s) 0ul i in
+                        let s2 = slice (as_seq h0 s) i (i +^ l) in
+                        let s2' = slice (as_seq h1 s) i (i +^ l) in
+                        let s3 = slice (as_seq h0 s) (i +^ l) ls in
+                        let s3' = slice (as_seq h1 s) (i +^ l) ls in
+                        s1 == s1' /\ s3 == s3' /\ s2' = f l s2)))
+
+
+let update_slice_st_f s ls i l =
+//  (**) let h0 = ST.get () in
+     let s1 = Buffer.sub s 0ul i in
+//  (**) let h1 = ST.get () in
+//  (**) assert(as_seq h1 s1 == as_seq h0 s1);
+    let s2 = Buffer.sub s i l in
+//  (**) let h2 = ST.get () in
+    let s3 = Buffer.sub s (i +^ l) (ls -^ i -^ l) in
+//  (**) let h3 = ST.get () in
+//  (**) assert(as_seq h3 s1 == as_seq h0 s1);
+    f_st s2 l
+//  (**) let h4 = ST.get () in
+//  (**) assert(as_seq h4 s2 == f #UInt8.t l(as_seq h3 s2))
